code/hash/Hacl.Test.Blake2s.fst
@@ -54,7 +54,7 @@ let main () =
   C.String.print (C.String.of_literal "\nTEST 1\n");
   let test1_result : lbuffer uint8 (size_v test1_expected_len) = create #uint8 (size 32) (u8 0) in
 
-  Hacl.Impl.Blake2s.blake2s #_ #_ #_ test1_result test1_plaintext test1_plaintext_len test1_empty_len empty test1_expected_len;
+  Hacl.Impl.Blake2s.blake2s #_ #_ #_ test1_result test1_plaintext test1_plaintext_len empty test1_empty_len test1_expected_len;
   (* Hacl.Impl.Blake2s.blake2s test1_plaintext_len test1_plaintext test1_empty_len empty test1_expected_len test1_result; *)
 
   Lib.Print.print_compare_display test1_expected_len test1_result test1_expected;
@@ -82,7 +82,7 @@ let main () =
 
   (* C.String.print (C.String.of_literal "\nTEST 2\n"); *)
   (* let test2_result : lbuffer uint8 (size_v test2_expected_len) = create #uint8 (size 32) (u8 0) in *)
-  (* Hacl.Impl.Blake2s.blake2s test2_plaintext_len test2_plaintext test2_key_len test2_key test2_expected_len test2_result; *)
+  (* Hacl.Impl.Blake2s.blake2s test2_plaintext_len test2_plaintext test2_key test2_key_len test2_expected_len test2_result; *)
 
   (* Display the result *)
   (* Lib.Print.print_compare_display test2_expected_len test2_result test2_expected; *)
